ParDB instances and type system specification

FOmegaC/SpecSyntax.v
@@ -1,4 +1,7 @@
+
 Require Export ParDB.Spec.
+Require Export ParDB.Lemmas.
+Require Export ParDB.Inst.
 
 Implicit Types x y α β c : Ix.
 
@@ -9,29 +12,30 @@ Inductive Kind : Type :=
 Implicit Types k : Kind.
 
 Inductive Tm : Type :=
-  | var    x
+  | var      x
   (**********************)
-  | absee  (τ e: Tm)
-  | absτe  k (e: Tm)
-  | absγe  (τ1 τ2 e : Tm)
-  | appee  (e1 e2 : Tm)
-  | appeτ  (e τ: Tm)
-  | appeγ  (e γ: Tm)
-  | cast   (e γ: Tm)
+  | absee    (τ e: Tm)
+  | absτe    k (e: Tm)
+  | absγe    (τ1 τ2: Tm) k (e : Tm)
+  | appee    (e1 e2 : Tm)
+  | appeτ    (e τ: Tm)
+  | appeγ    (e γ: Tm)
+  | cast     (e γ: Tm)
   (**********************)
-  | absττ  k (τ: Tm)
-  | appττ  (τ1 τ2: Tm)
-  | arree  (τ1 τ2: Tm)
-  | arrτe  k (τ: Tm)
-  | arrγe  (τ1 τ2 τ3: Tm)
+  | absττ    k (τ: Tm)
+  | appττ    (τ1 τ2: Tm)
+  | arree    (τ1 τ2: Tm)
+  | arrτe    k (τ: Tm)
+  | arrγe    (τ1 τ2: Tm) k (τ3: Tm)
   (**********************)
-  | γabsττ k (γ: Tm)
-  | γappττ (γ1 γ2: Tm)
-  | γarree (γ1 γ2: Tm)
-  | γarrτe k (γ: Tm)
-  | γarrγe (τ1 τ2 γ: Tm)
-  | γsym   (γ: Tm)
-  | γtrans (γ1 γ2: Tm).
+  | γabsττ   k (γ: Tm)
+  | γappττ   (γ1 γ2: Tm)
+  | γarree   (γ1 γ2: Tm)
+  | γarrτe   k (γ: Tm)
+  | γarrγe   (τ1 τ2 γ: Tm)
+  | γbeta    (γ1 γ2: Tm)
+  | γsym     (γ: Tm)
+  | γtrans   (γ1 γ2: Tm).
 
 Implicit Types t e τ γ : Tm.
 
@@ -39,11 +43,13 @@ Inductive Env : Set :=
   | nil
   | evar (Γ: Env) τ
   | τvar (Γ: Env) k
-  | γvar (Γ: Env) τ τ.
+  | γvar (Γ: Env) τ1 τ2 k.
 
-Notation "Γ ▻ τ"       := (evar Γ τ) (at level 55, left associativity).
-Notation "Γ ► k"       := (τvar Γ k) (at level 55, left associativity).
-Notation "Γ ◅ τ1 ~ τ2" := (γvar Γ τ1 τ2) (at level 55, left associativity).
+Implicit Types Γ : Env.
+
+Notation "Γ ▻ τ"           := (evar Γ τ) (at level 55, left associativity).
+Notation "Γ ► k"           := (τvar Γ k) (at level 55, left associativity).
+Notation "Γ ◅ τ1 ~ τ2 ∷ k" := (γvar Γ τ1 τ2 k) (at level 55, left associativity).
 
 Section DeBruijn.
 
@@ -55,29 +61,102 @@ Section DeBruijn.
 
   Fixpoint apTm (ζ: Sub X) (t: Tm) {struct t} : Tm :=
     match t with
-      | var x          => lift (ζ x)
+      | var x            =>  lift (ζ x)
       (**************************************************************)
-      | absee τ e      => absee (apTm ζ τ) (apTm ζ↑ e)
-      | absτe k e      => absτe k (apTm ζ↑ e)
-      | absγe τ1 τ2 e  => absγe (apTm ζ τ1) (apTm ζ τ2) (apTm ζ↑ e)
-      | appee e1 e2    => appee (apTm ζ e1) (apTm ζ e2)
-      | appeτ e τ      => appeτ (apTm ζ e) (apTm ζ τ)
-      | appeγ e γ      => appeγ (apTm ζ e) (apTm ζ γ)
-      | cast e γ       => cast (apTm ζ e) (apTm ζ γ)
+      | absee τ e        =>  absee τ[ζ] e[ζ↑]
+      | absτe k e        =>  absτe k e[ζ↑]
+      | absγe τ1 τ2 k e  =>  absγe τ1[ζ] τ2[ζ] k e[ζ↑]
+      | appee e1 e2      =>  appee e1[ζ] e2[ζ]
+      | appeτ e τ        =>  appeτ e[ζ] τ[ζ]
+      | appeγ e γ        =>  appeγ e[ζ] γ[ζ]
+      | cast e γ         =>  cast e[ζ] γ[ζ]
       (**************************************************************)
-      | absττ k τ      => absττ k (apTm ζ↑ τ)
-      | appττ τ1 τ2    => appττ (apTm ζ τ1) (apTm ζ τ2)
-      | arree τ1 τ2    => arree (apTm ζ τ1) (apTm ζ↑ τ2)
-      | arrτe k τ      => arrτe k (apTm ζ↑ τ)
-      | arrγe τ1 τ2 τ3 => arrγe (apTm ζ τ1) (apTm ζ τ2) (apTm ζ τ3)
+      | absττ k τ        =>  absττ k τ[ζ↑]
+      | appττ τ1 τ2      =>  appττ τ1[ζ] τ2[ζ]
+      | arree τ1 τ2      =>  arree τ1[ζ] τ2[ζ]
+      | arrτe k τ        =>  arrτe k τ[ζ↑]
+      | arrγe τ1 τ2 k τ3 =>  arrγe τ1[ζ] τ2[ζ] k τ3[ζ↑]
       (**************************************************************)
-      | γabsττ k γ     => γabsττ k (apTm ζ↑ γ)
-      | γappττ γ1 γ2   => γappττ (apTm ζ γ1) (apTm ζ γ2)
-      | γarree γ1 γ2   => γarree (apTm ζ γ1) (apTm ζ γ2)
-      | γarrτe k γ     => γarrτe k (apTm ζ↑ γ)
-      | γarrγe τ1 τ2 γ => γarrγe (apTm ζ τ1) (apTm ζ τ2) (apTm ζ γ)
-      | γsym γ         => γsym (apTm ζ γ)
-      | γtrans γ1 γ2   => γtrans (apTm ζ γ1) (apTm ζ γ2)
-    end.
+      | γabsττ k γ       =>  γabsττ k γ[ζ↑]
+      | γappττ γ1 γ2     =>  γappττ γ1[ζ] γ2[ζ]
+      | γarree γ1 γ2     =>  γarree γ1[ζ] γ2[ζ]
+      | γarrτe k γ       =>  γarrτe k γ[ζ↑]
+      | γarrγe τ1 τ2 γ   =>  γarrγe τ1[ζ] τ2[ζ] γ[ζ↑]
+      | γbeta γ1 γ2      =>  γbeta γ1[ζ] γ2[ζ]
+      | γsym γ           =>  γsym γ[ζ]
+      | γtrans γ1 γ2     =>  γtrans γ1[ζ] γ2[ζ]
+    end
+  where "t '[' ζ ']'" := (apTm ζ t).
 
 End DeBruijn.
+
+Instance vrTm : Vr Tm := {| vr := var |}.
+Proof. inversion 1; auto. Defined.
+
+Module TmKit <: Kit.
+
+  Definition TM := Tm.
+  Definition inst_vr := vrTm.
+
+  Local Ltac refold :=
+    match goal with
+      | [ |- context[apTm ?ξ ?t] ] =>
+        change (apTm ξ t) with t[ξ]
+    end.
+
+  Local Ltac crush :=
+    intros; cbn in * |-;
+    repeat
+      (cbn;
+       repeat crushDbSyntaxMatchH;
+       repeat crushDbLemmasMatchH;
+       rewrite ?comp_up, ?up_liftSub, ?up_comp_lift;
+       repeat refold);
+    auto.
+
+  Local Ltac derive :=
+    crush; f_equal; crush.
+
+  Section Application.
+
+    Context {Y: Type}.
+    Context {vrY : Vr Y}.
+    Context {wkY: Wk Y}.
+    Context {liftY: Lift Y Tm}.
+
+    Global Instance inst_ap : Ap Tm Y := {| ap := apTm |}.
+    Proof. induction x; derive. Defined.
+
+    Global Instance inst_ap_vr : LemApVr Tm Y := {}.
+    Proof. reflexivity. Qed.
+
+  End Application.
+
+  Instance inst_ap_inj: LemApInj Tm Ix := {}.
+  Proof.
+    intros m Inj_m x. revert m Inj_m.
+    induction x; destruct y; simpl; try discriminate;
+    inversion 1; subst; f_equal; eauto using InjSubIxUp.
+  Qed.
+
+  Instance inst_ap_comp (Y Z: Type)
+    {vrY: Vr Y} {wkY: Wk Y} {liftY: Lift Y Tm}
+    {vrZ: Vr Z} {wkZ: Wk Z} {liftZ: Lift Z Tm}
+    {apYZ: Ap Y Z} {compUpYZ: LemCompUp Y Z}
+    {apLiftYTmZ: LemApLift Y Z Tm} :
+    LemApComp Tm Y Z := {}.
+  Proof. induction x; derive. Qed.
+
+  Instance inst_ap_liftSub (Y: Type)
+    {vrY: Vr Y} {wkY: Wk Y} {liftY: Lift Y Tm} :
+    LemApLiftSub Tm Y := {}.
+  Proof. induction t; derive. Qed.
+
+  Lemma inst_ap_ixComp (t: Tm) :
+    ∀ (ξ: Sub Ix) (ζ: Sub Tm), t[ξ][ζ] = t[⌈ξ⌉ >=> ζ].
+  Proof. induction t; derive. Qed.
+
+End TmKit.
+
+Module InstTm := Inst TmKit.
+Export InstTm. (* Export for shorter names. *)
